Add proofs on [Records] (wip).

test/coq/records/records_proof.v
@@ -6,7 +6,36 @@ Import uPred.
 
 From osiris Require Import osiris.
 From osiris.libs Require Import Stdlib.
-From test Require Import records.
+From test.records Require Import records records_code.
+
+(* -------------------------------------------------------------------------- *)
+
+(* Table of content of the file:
+   1. Definition of an instance of [Encode] for the a Coq-type representing
+      OCaml records of type [{ b: bool; i: int }].
+   2. Definitions of values (of type [val]) representing OCaml values appearing
+      in the proofs.
+   3. Definitions of specifications for elements of the module.
+   4. Proofs that each function body respects its specification
+      (These are used in the caller-side-reasoning style proof below.)
+   5. Proofs that each function respects its specification
+      (These are used in the callee-side-reasoning style proof below.)
+   6. Proof of the module (Caller-side reasoning).
+   7. Proof of the module (Callee-side reasoning).
+   8. Direct proof of the module (in one lemma).
+
+Efficiency of 4--5: TODO.
+
+Efficiency of 6--8: TODO. *)
+
+(* -------------------------------------------------------------------------- *)
+
+(* Make sure that the modules [Record] (defined in [records.v]) and
+   [opacified_Records] (defined in [records_code.v]) coincide. *)
+Goal opacified_Records = Records.
+Proof. reflexivity. Qed.
+
+(* -------------------------------------------------------------------------- *)
 
 Local Transparent eval. (* TODO. *)
 
@@ -16,7 +45,7 @@ Context `{!osirisGS_gen hlc Σ}.
 
 (* -------------------------------------------------------------------------- *)
 
-(* Local defintiion of the record type used in [records.ml]. *)
+(* (1) Local defintion of the record type used in [records.ml]. *)
 
 Record R :=
   { b: bool ;
@@ -32,14 +61,14 @@ Local Instance r_encode : Encode R :=
 
 (* -------------------------------------------------------------------------- *)
 
-(* Definition of some values; useful to write the specs below. *)
+(* (2) Definition of some values; useful to write the specs below. *)
 Definition enc_r_elt : val := #{| b := true; i := 10 |}.
 Definition enc_r_elt' : val := #{|b := false; i := 10|}.
 Definition enc_lily : val := # [enc_r_elt; enc_r_elt'].
 
 (* -------------------------------------------------------------------------- *)
 
-(* Definition of the specifications. *)
+(* (3) Definition of specifications. *)
 
 (* [is_equal] asserts the equality of two values. *)
 Definition is_equal v : val → iProp Σ :=
@@ -64,17 +93,14 @@ Definition r_val_pure (r: R) : Z :=
   end.
 
 Definition r_val_spec (r_val: val): iProp Σ :=
-  ∀ (i: Z) (b: bool),
-    let r := {| b := b; i := i |} in
+  ∀ (r: R),
     WP call r_val #r
        {{ λ result, is_equal result #(r_val_pure r) }}.
 
 Definition sum_pure (r1 r2: R) : Z :=
   r_val_pure r1 + r_val_pure r2.
 Definition sum_spec (vsum: val) : iProp Σ :=
-  ∀ (b1 b2: bool) (i1 i2: Z),
-    let r1 := {| b := b1; i := i1 |} in
-    let r2 := {| b := b2; i := i2 |} in
+  ∀ (r1 r2 : R),
     WP call vsum #r1 {{
           λ vpart,
           WP call vpart #r2 {{
@@ -83,11 +109,342 @@ Definition sum_spec (vsum: val) : iProp Σ :=
 
 (* -------------------------------------------------------------------------- *)
 
-(* Proof of the module [Records] in which the function bodies have not been
-   turned opaque. *)
+(* Staging area. *)
 
+Opaque
+  r_elt_expr
+  flip_body flip_function
+  lily_expr
+  r_val_body r_val_function
+  sum_body sum_function
+.
+
+(* [explicit name] unfolds [name], even if transparent. *)
+Ltac explicit name :=
+  with_strategy transparent [ name ] unfold name.
+
+(* [wp_simp] simplifies the element of type [free A] we are working on. *)
 Ltac wp_simp :=
-  progress (iApply wp_simp; first by simp); wp.
+  progress (iApply wp_simp; first by simp).
+
+Arguments String.eqb !s1 !s2 : simpl nomatch. (* TODO *)
+
+(* -------------------------------------------------------------------------- *)
+
+(* (4) Specifications of function bodies. *)
+
+Lemma r_elt_spec η :
+  simp (eval η r_elt_expr) (ret enc_r_elt).
+Proof.
+  explicit r_elt_expr.
+  simp.
+Qed.
+
+Lemma flip_body_spec :
+  ∀ (r: var) (b: bool) (i: Z) η,
+    lookup_name η "Stdlib" = ret Stdlib →
+    lookup_name η r = ret #{| b := b; i := i |} →
+    simp (eval η (flip_body r))
+         (ret #{| b := negb b; i := i |}).
+Proof.
+  explicit flip_body.
+  intros r [] i η Hstdlib Hr; simp;
+    (eapply prove_simp_bind;
+     [ explicit call; simp
+     | simp ]).
+Qed.
+
+Lemma lily_body_spec η η' :
+  let clo_flip := VClo η' (AnonFun1Pat (PVar "r") (flip_body "r")) in
+  (* Requirements of [flip_body_spec]. *)
+  lookup_name η' "Stdlib" = ret Stdlib →
+  (* Requirements of [lily_body_spec] *)
+  lookup_name η "r_elt" = ret enc_r_elt →
+  lookup_name η "flip" = ret clo_flip →
+  lookup_name η "Stdlib" = ret Stdlib →
+  (* Actual spec. *)
+  simp (eval η lily_expr) (ret enc_lily).
+Proof.
+  intros ? ? Hrelt Hflip Hstdlib.
+  explicit lily_expr.
+  simp.
+  rewrite Hrelt; simp.
+  eapply prove_simp_bind.
+  { explicit call.
+    simpl. simp.
+    explicit concatenating.
+    eapply flip_body_spec; try done.
+    (* FIXME. *)
+    instantiate (1 := 10). instantiate (1 := true).
+    done. }
+  simp.
+Qed.
+
+Lemma r_val_body_spec η (r: R) (rvar: var) :
+  lookup_name η "Stdlib" = ret Stdlib →
+  lookup_name η rvar = ret #r →
+  simp (eval η (r_val_body rvar)) (ret #(r_val_pure r)).
+Proof.
+  explicit r_val_body.
+  intros??. destruct (r.(b)) eqn:E;
+    simp; rewrite E; simp; simp_continue;
+    rewrite /r_val_pure E; simp. explicit call.
+  simp.
+  rewrite int.mul_repr_repr
+          int.sub_repr_repr.
+  simp.
+Qed.
+
+Lemma sum_body_spec η (r1 r2: R):
+  lookup_name η "r1" = ret #r1 →
+  lookup_name η "r2" = ret #r2 →
+  lookup_name η "Stdlib" = ret Stdlib →
+  lookup_name η "r_val" = (eval η (EAnonFun $ AnonFun "r" (r_val_body "r"))) →
+  simp (eval η (sum_body "r1" "r2")) (ret #(sum_pure r1 r2)).
+Proof.
+  intros H1 H2 H3 H4.
+  explicit sum_body. simp. rewrite H1 H2 H4. explicit call.
+  cbn.
+  etransitivity; first (apply SimpPar; simp).
+  etransitivity;
+    first (apply SimpPar;
+           [ apply simp_bind; by apply r_val_body_spec
+           | solve [simp] ]).
+  simp.
+  etransitivity; first (apply simp_bind; by apply r_val_body_spec).
+  simp.
+  unfold sum_pure.
+  rewrite int.add_repr_repr.
+  reflexivity.
+Qed.
+
+(* -------------------------------------------------------------------------- *)
+
+(* (5) Specifications of functions. *)
+
+Lemma flip_function_spec :
+  ∀ η,
+    lookup_name η "Stdlib" = Ret Stdlib →
+    ⊢ ∃ vflip,
+    ⌜simp (eval η flip_function) (Ret vflip)⌝
+          ∗ flip_spec vflip.
+Proof.
+  intros? H1.
+  iExists _.
+  iSplit; first (iPureIntro; by simp).
+  explicit flip_body.
+  iIntros (b i).
+  wp_call. wp_continue.
+  rewrite H1. wp.
+  simpl (build _ _). wp.
+  iPureIntro. reflexivity.
+Qed.
+
+Lemma r_val_function_spec η :
+  lookup_name η "Stdlib" = Ret Stdlib →
+  ⊢ ∃ vr_val,
+    ⌜simp (eval η r_val_function) (Ret vr_val)⌝
+          ∗ r_val_spec vr_val.
+Proof.
+  intros H1.
+  iExists _.
+  iSplit; first (iPureIntro; by simp).
+  by iIntros (r); explicit r_val_body; explicit r_val_pure;
+  wp_call; destruct (b r); do 2 wp_continue; [ rewrite H1; wp | ].
+Qed.
+
+Lemma sum_function_spec η vr_val :
+  lookup_name η "Stdlib" = Ret Stdlib →
+  lookup_name η "r_val" = Ret vr_val →
+  (* TODO: add the requirements of [sum_function]. *)
+  ⊢ □ r_val_spec vr_val -∗
+    ∃ vsum,
+      ⌜simp (eval η sum_function) (Ret vsum)⌝ ∗ sum_spec vsum.
+Proof.
+  iIntros(??) "#Hr_val".
+  iExists _.
+  iSplit; first (iPureIntro; by simp).
+  iIntros (r1 r2).
+  explicit sum_body.
+  wp_call; do 2 wp_continue.
+  wp_simp.
+  wp_par.
+  { wp_use "Hr_val". iIntros (?<-). wp_call. wp_set_postcondition. }
+  { wp_use "Hr_val". }
+  iIntros (??-><-). wp.
+  wp_call.
+
+  explicit sum_pure.
+  iPureIntro. rewrite int.add_repr_repr. reflexivity.
+Qed.
+
+(* -------------------------------------------------------------------------- *)
+
+(* (6) The following proof is written in caller-reasoning style. It exploits the
+   above proofs on the function bodies. *)
+
+Ltac wp_simp_using H :=
+  iApply wp_simp; [ by apply H | wp ].
+
+Transparent
+  flip_function
+  r_val_function
+  sum_function
+.
+
+Goal
+    let Λ :=
+      [
+        ("is_odd", trivial_spec) ;
+        ("is_odd_naive", trivial_spec) ;
+        ("sum", sum_spec) ;
+        ("r_val", r_val_spec) ;
+        ("lily", is_equal enc_lily) ;
+        ("flip", flip_spec) ;
+        ("r_elt", is_equal enc_r_elt)
+    ]
+  in
+  let η := EnvCons "Stdlib" Stdlib $
+           EnvNil in
+  ⊢ WP eval_mexpr η opacified_Records {{ module_spec Λ }}.
+Proof.
+  (* Proof using [simp]. *)
+  intros ??. wp.
+  simpl (build _ _). wp.
+
+  wp_simp_using r_elt_spec.
+  wp_specify "r_elt" (is_equal enc_r_elt); first done.
+  iIntros(?->). wp_continue.
+
+  wp_continue.
+  iApply wp_simp.
+  { by eapply lily_body_spec; try done. }
+
+  wp. wp_continue.
+
+  (* [r_val] has the expected value. *)
+  wp_specify "r_val" r_val_spec.
+  { iIntros (r). explicit r_val_pure; destruct (b r) eqn:E;
+      wp_call; wp_continue;
+      (iApply wp_simp; first eapply r_val_body_spec); try done;
+      explicit r_val_pure; rewrite E; by wp. }
+  iIntros (r_val) "#Hr_val". wp_continue.
+
+
+  (* [sum] is given the trivial spec for now. *)
+  wp_continue.
+
+  (* [is_odd_naive] is given the trivial spec for now. *)
+  wp_specify "is_odd_naive" trivial_spec; first done.
+  iIntros (is_odd_naive) "#His_odd_naive". wp_continue.
+
+  (* [is_odd] is given the trivial spec for now. *)
+  wp_specify "is_odd" trivial_spec; first done.
+  iIntros (is_odd) "#His_odd". wp_continue.
+
+
+  lazymatch goal with
+  | |- environments.envs_entails _ (?φ (VStruct ?η)) =>
+      iExists _; iSplit ; first (iPureIntro; reflexivity)
+  end.
+  cbn; repeat iSplitL; try (iExists _; iSplit; first done); try done.
+  { (* Proof of the [sum] function.*)
+    iIntros(r1 r2).
+    wp_call. wp_continue. wp_continue.
+    wp_par.
+    - wp_use "Hr_val".
+      iIntros(?<-).
+      wp_call. wp_set_postcondition.
+    - wp_use "Hr_val".
+    - iIntros (v1 v2 -> <-). wp.
+      wp_call.
+      iPureIntro. unfold sum_pure;
+        destruct (b r1), (b r2); cbn;
+        by rewrite int.add_repr_repr. }
+  { (* Proof of the [flip] function. *)
+    iIntros(??); wp_call. wp_continue.
+    by wp_simp_using flip_body_spec. }
+Time Qed.
+
+Opaque
+  flip_function
+  r_val_function
+  sum_function
+.
+
+(* -------------------------------------------------------------------------- *)
+
+
+(* (7) The following proof is written in callee-reasoning style. It exploits the
+   above proofs on the function expressions. *)
+
+Goal
+    let Λ :=
+      [
+        ("is_odd", trivial_spec) ;
+        ("is_odd_naive", trivial_spec) ;
+        ("sum", sum_spec) ;
+        ("r_val", r_val_spec) ;
+        ("lily", is_equal enc_lily) ;
+        ("flip", flip_spec) ;
+        ("r_elt", is_equal enc_r_elt)
+    ]
+  in
+  let η := EnvCons "Stdlib" Stdlib $
+           EnvNil in
+  ⊢ WP eval_mexpr η opacified_Records {{ module_spec Λ }}.
+Proof.
+  intros??.
+  wp.
+
+  wp_simp_using r_elt_spec.
+  wp_specify "r_elt" (is_equal enc_r_elt); first done.
+  iIntros (?->). wp_continue.
+
+  lazymatch goal with
+  | |- environments.envs_entails _ (wp _ _ (eval ?η flip_function) _) =>
+      iPoseProof (flip_function_spec η)
+      as "[%vflip [%Hflip_simp #Hflip_spec]]";
+      first reflexivity
+  end.
+  wp_simp_using Hflip_simp. wp_continue.
+
+  explicit lily_expr.
+  wp. wp_simp. wp.
+
+  replace (VRecord _) with #{| b := true ;i := 10|}; last reflexivity.
+  wp_use "Hflip_spec". iIntros(?<-). wp.
+  wp_continue.
+
+
+  lazymatch goal with
+  | |- environments.envs_entails _ (wp _ _ (eval ?η r_val_function) _) =>
+      iPoseProof (r_val_function_spec η)
+      as "[%vr_val [%Hr_val_simp #Hr_val_spec]]";
+      first reflexivity
+  end.
+  wp_simp_using Hr_val_simp. wp_continue.
+
+  lazymatch goal with
+  | |- environments.envs_entails _ (wp _ _ (eval ?η sum_function) _) =>
+      iPoseProof ((sum_function_spec η) with "Hr_val_spec")
+      as "[%vsum [%Hsum_simp #Hsum_spec]]";
+      try reflexivity
+  end.
+  wp_simp_using Hsum_simp. wp_continue.
+
+  wp_specify "is_odd_naive" trivial_spec; first done.
+  iIntros (?) "?". wp_continue.
+  wp_specify "is_odd" trivial_spec; first done.
+  iIntros (?) "?". wp_continue.
+
+  wp_module_spec.
+Time Qed.
+
+(* -------------------------------------------------------------------------- *)
+
+(* (8) Proof of the module [Records] in which the function bodies have not been
+   turned opaque. *)
 
 Lemma Records_spec :
     let Λ :=
@@ -120,7 +477,7 @@ Proof.
   iIntros (flip) "#Hflip". wp_continue.
 
   (* [flip] is applied to [r_elt]. *)
-  wp_simp.
+  wp_simp. wp.
   replace
     (VRecord (EnvCons "b" VTrue (EnvCons "i" (VInt (int.repr 10)) EnvNil)))
     with #{| b := true; i := 10 |}; last reflexivity.
@@ -137,7 +494,7 @@ Proof.
 
   (* [r_val] has the expected value. *)
   wp_specify "r_val" r_val_spec.
-  { iIntros (i [|]).
+  { iIntros ([[|] i]).
     (* Case: [b] is true. *)
     { wp_call. by do 2 wp_continue. }
     { wp_call. by do 2 wp_continue. } }
@@ -146,12 +503,17 @@ Proof.
 
   (* [sum] is given the trivial spec for now. *)
   wp_specify "sum" sum_spec.
-  { iIntros(b1 b2 i1 i2). wp_call. do 2 wp_continue.
+  { iIntros([b1 i1] [b2 i2]). wp_call. do 2 wp_continue.
     wp.
-    wp_par.
+    wp_simp.
+    wp_par;
+    (replace (VRecord (EnvCons "b" (VBool b1) $ EnvCons "i" (VInt (int.repr i1)) EnvNil))
+      with (#{| b:=b1; i:= i1|}); last reflexivity);
+    (replace (VRecord (EnvCons "b" (VBool b2) $ EnvCons "i" (VInt (int.repr i2)) EnvNil))
+      with (#{| b:=b2; i:= i2|}); last reflexivity).
     2: by wp_use "Hr_val".
     { wp_use "Hr_val". iIntros(?<-).
-      apply tc_change_goal. iIntros (vpartial).
+      wp. iIntros (vpartial).
       iIntros "H"; iExact "H". }
     { iIntros (v1 v2) "Hadd <-".
       wp. iApply (wp_covariant with "Hadd").
@@ -170,362 +532,4 @@ Proof.
 
   (* Every spec has been proven: [wp_module_spec] can finish the proof. *)
   wp_module_spec.
-Time Qed.
-
-(* -------------------------------------------------------------------------- *)
-
-(* Definition of function bodies.  These are the bodies of functions which will
-   be proven. The goal is to see if it is easier to specify each of these bodies
-   before the main proof. *)
-
-(* Body of [flip]. *)
-Definition flip_body (r: var) :expr :=
-  ERecordUpdate (EPath (PathBase r))
-                (FECons
-                   "b"
-                   (EApp (EPath (PathDot (PathBase "Stdlib") "not"))
-                         (ERecordAccess (EPath (PathBase r)) "b")) FENil).
-
-Definition is_odd_body : expr :=
-  EApp
-    (EApp (EPath (PathDot (PathBase "Stdlib") "=")) $
-          EApp (
-            EApp (EPath (PathDot (PathBase "Stdlib")
-                                 "mod")) $
-                 EPath (PathBase "n"))
-          (EInt 2))
-    (EInt 0).
-
-Definition is_odd_naive_body : expr :=
-  ESeq
-    (EAssert $
-             EApp
-             (EApp (EPath (PathDot (PathBase "Stdlib") ">="))
-                   (EPath (PathBase "n"))) $
-             EInt 0) $
-    EIfThenElse (
-      EApp
-        (EApp (EPath (PathDot (PathBase "Stdlib") ">"))
-              (EPath (PathBase "n")))
-        (EInt 1))
-    (EApp (EPath (PathBase "is_odd_naive")) $
-          EApp
-          (EApp (EPath (PathDot (PathBase "Stdlib")
-                                "-"))
-                (EPath (PathBase "n")))
-          (EInt 2)) $
-    EIfThenElse (
-      EApp (
-          EApp (EPath (PathDot (PathBase "Stdlib")
-                               "="))
-               (EPath (PathBase "n")))
-           (EInt 0))
-    (EData "false" (ETuple ENil))
-    (EData "true" (ETuple ENil))
-.
-
-Definition sum_body : expr :=
-  EApp (
-      EApp (EPath (PathDot (PathBase "Stdlib") "+")) $
-           EApp (EPath (PathBase "r_val"))
-           (EPath (PathBase "r1"))
-    ) $
-       EApp (EPath (PathBase "r_val"))
-       (EPath (PathBase "r2"))
-.
-Definition r_elt_body : expr :=
-  ERecord (
-      FECons "i"
-             (EInt 10)
-              (FECons "b" (EData "true" (ETuple ENil)) FENil)).
-
-Definition lily_body : expr :=
-  EData "::"
-        $ ETuple  $
-        ECons (EPath (PathBase "r_elt")) $
-        ECons
-        (EData "::"
-               (ETuple $
-                       ECons (
-                         EApp (EPath (PathBase "flip"))
-                              (EPath (PathBase "r_elt"))) $
-                       ECons (EData "[]" (ETuple ENil))
-                       ENil))
-        ENil
-.
-
-Definition r_val_body (r: var) : expr :=
-  EMatch (ERecordAccess (EPath (PathBase r)) "b") $
-         MkBranches
-         [ Branch (PBool true) $
-                  EApp (
-                    EApp (EPath (PathDot (PathBase "Stdlib") "-"))
-                         (EApp (
-                              EApp (EPath (PathDot (PathBase "Stdlib")
-                                                   "*"))
-                                   (ERecordAccess (EPath (PathBase r)) "i")
-                            )
-                               (EInt 2)
-                         )
-                  )
-                  (EInt 1)
-           ; Branch (PBool false)
-                    (ERecordAccess (EPath (PathBase r)) "i")
-         ]
-.
-
-Definition Opacified_Records : mexpr :=
-  MkStruct [
-      ILet (Binding1 (PVar "r_elt") r_elt_body)
-      ;
-      ILet (Binding1 (PVar "flip")
-                     (EAnonFun (
-                          AnonFun1Pat (PVar "r")
-                                      (flip_body "r"))))
-      ;
-      ILet (Binding1 (PVar "lily") lily_body)
-      ;
-      ILet $
-          Binding1 (PVar "r_val") $
-                   EAnonFun ( AnonFun1Pat (PVar "r") (r_val_body "r"))
-      ;
-      ILet $
-           Binding1 (PVar "sum") $
-           EAnonFun $
-           AnonFun1Pat (PVar "r1") $
-           EAnonFun $
-           AnonFun1Pat (PVar "r2") $
-           sum_body
-      ;
-      ILetRec $
-          RecBiCons
-          (RecBinding "is_odd_naive" $
-           AnonFun1Pat (PVar "n") $
-           is_odd_naive_body)
-          RecBiNil
-      ;
-      ILet $
-           Binding1 (PVar "is_odd") $
-           EAnonFun $
-           AnonFun1Pat (PVar "n") $
-           is_odd_body
-    ].
-
-Lemma Records_eq :
-  Records =
-    Opacified_Records.
-Proof. reflexivity. Qed.
-
-
-(* Bodies are turned opaque. *)
-Opaque
-  flip_body
-  lily_body
-  is_odd_body
-  is_odd_naive_body
-  r_val_body
-.
-
-(* -------------------------------------------------------------------------- *)
-
-(* Specifications of function bodies. *)
-
-Lemma flip_body_spec :
-  ∀ (r: var) (b: bool) (i: Z) η,
-    lookup_name η "Stdlib" = ret Stdlib →
-    lookup_name η r = ret #{| b := b; i := i |} →
-    simp (eval η (flip_body r))
-         (ret #{| b := negb b; i := i |}).
-Proof.
-  with_strategy transparent [flip_body] unfold flip_body.
-  intros r [] i η Hstdlib Hr; simp;
-    (eapply prove_simp_bind;
-     [ with_strategy transparent [ Stdlib__not ] unfold Stdlib__not;
-       with_strategy transparent [ call ] unfold call; simp
-     | simp ]).
-Qed.
-
-Lemma lily_body_spec η η' :
-  let clo_flip := VClo η' (AnonFun1Pat (PVar "r") (flip_body "r")) in
-  (* Thefollowing is required to use [flip_body_spec]. *)
-  lookup_name η' "Stdlib" = ret Stdlib →
-  lookup_name η "r_elt" = ret enc_r_elt →
-  lookup_name η "flip" = ret clo_flip →
-  lookup_name η "Stdlib" = ret Stdlib →
-  simp (eval η lily_body) (ret enc_lily).
-Proof.
-  intros ? ? Hrelt Hflip Hstdlib.
-  with_strategy transparent [lily_body] unfold lily_body.
-  simp.
-  rewrite Hrelt; simp.
-  eapply prove_simp_bind.
-  { with_strategy transparent [call] unfold call.
-    simpl. simp.
-    with_strategy transparent [ concatenating ] (unfold concatenating at 1).
-    eapply flip_body_spec; try done.
-    (* FIXME. *)
-    instantiate (1 := 10). instantiate (1 := true).
-    done. }
-  simp.
-Qed.
-
-Ltac rew name :=
-  with_strategy transparent [ name ] unfold name.
-
-Arguments String.eqb !s1 !s2 : simpl nomatch. (* TODO *)
-Lemma r_val_body_spec η (r: R) (rvar: var) :
-  lookup_name η "Stdlib" = ret Stdlib →
-  lookup_name η rvar = ret #r →
-  simp (eval η (r_val_body rvar)) (ret #(r_val_pure r)).
-Proof.
-  rew r_val_body.
-  intros??. destruct (r.(b)) eqn:E;
-    simp; rewrite E; simp; simp_continue;
-    rewrite /r_val_pure E; simp.
-  rew Stdlib__mul. rew Stdlib__sub. rew call.
-  simp.
-  rewrite int.mul_repr_repr
-          int.sub_repr_repr.
-  simp.
-Qed.
-
-Global Instance simp_reflexive {A} : Reflexive (@simp A) :=
-  SimpReflexive.
-Global Instance simp_transitive {A} : Transitive (@simp A) :=
-  SimpTransitive.
-
-Lemma sum_body_spec η (r1 r2: R):
-  lookup_name η "r1" = ret #r1 →
-  lookup_name η "r2" = ret #r2 →
-  lookup_name η "Stdlib" = ret Stdlib →
-  lookup_name η "r_val" = (eval η (EAnonFun $ AnonFun "r" (r_val_body "r"))) →
-  simp (eval η sum_body) (ret #(sum_pure r1 r2)).
-Proof.
-  intros H1 H2 H3 H4.
-  rew sum_body. simp. rewrite H1 H2 H4. rew call.
-  cbn.
-  etransitivity; first (apply SimpPar; simp).
-  etransitivity;
-    first (apply SimpPar;
-           [ apply simp_bind; by apply r_val_body_spec
-           | solve [simp] ]).
-  simp.
-  etransitivity; first (apply simp_bind; by apply r_val_body_spec).
-  simp.
-  unfold sum_pure.
-  rewrite int.add_repr_repr.
-  reflexivity.
-Qed.
-
-(* -------------------------------------------------------------------------- *)
-
-(* [wp] and [wp_continue] do *not* respect the opacity of the above expressions.
-   This is caused by [apply tc_change_goal] in [wp]which tries to simplify the
-   goal using any instance of [TC_change_goal]. *)
-
-Ltac wp' := wp.
-Ltac wp'_continue := wp_continue.
-
-Ltac wp :=
-  iStartProof; cbn;
-   repeat
-    lazymatch goal with
-    | |- environments.envs_entails _ (▷ _) => iNext
-    | _ => wp_step; try progress cbn
-    end.
-
-Ltac wp_continue :=
-  lazymatch goal with
-  | |- environments.envs_entails
-         _ (wp _ _ (concatenating eval _ _ ?δ) _) =>
-      with_strategy transparent [ concatenating ] (unfold concatenating at 1)
-  | |- environments.envs_entails
-         _ (wp _ _ (dconcatenating ?δ _) _) =>
-      with_strategy transparent [ dconcatenating ] (unfold dconcatenating at 1)
-  end; wp.
-
-Ltac wp_simp_using H :=
-  iApply wp_simp; [ by apply H | wp ].
-
-Lemma Records_spec_bodies :
-    let Λ :=
-      [
-        ("is_odd", trivial_spec) ;
-        ("is_odd_naive", trivial_spec) ;
-        ("sum", sum_spec) ;
-        ("r_val", r_val_spec) ;
-        ("lily", is_equal enc_lily) ;
-        ("flip", flip_spec) ;
-        ("r_elt", is_equal enc_r_elt)
-    ]
-  in
-  let η := EnvCons "Stdlib" Stdlib $
-           EnvNil in
-  ⊢ WP eval_mexpr η Records {{ module_spec Λ }}.
-Proof.
-  rewrite Records_eq.
-
-  (* Proof using [simp]. *)
-  intros ??. wp.
-  simpl (build _ _). wp.
-
-  wp_specify "r_elt" (is_equal enc_r_elt); first done.
-  iIntros(?->). wp_continue.
-
-  wp_continue.
-  iApply wp_simp.
-  { by eapply lily_body_spec; try done. }
-
-  wp. wp_continue.
-
-  (* [r_val] has the expected value. *)
-  wp_specify "r_val" r_val_spec.
-  { iIntros (i[|]).
-    (* Case: [b] is true. *)
-    { wp_call. wp'_continue.
-      iApply wp_simp; first eapply r_val_body_spec.
-      - done.
-      - by instantiate (1 := {| b := true; i := i |}).
-      - by wp. }
-    { wp_call. wp'_continue.
-      iApply wp_simp; first eapply r_val_body_spec.
-      - done.
-      - by instantiate (1 := {| b := false; i := i |}).
-      - by wp. } }
-  iIntros (r_val) "#Hr_val". wp_continue.
-
-
-  (* [sum] is given the trivial spec for now. *)
-  wp_continue.
-
-  (* [is_odd_naive] is given the trivial spec for now. *)
-  wp_specify "is_odd_naive" trivial_spec; first done.
-  iIntros (is_odd_naive) "#His_odd_naive". wp_continue.
-
-  (* [is_odd] is given the trivial spec for now. *)
-  wp_specify "is_odd" trivial_spec; first done.
-  iIntros (is_odd) "#His_odd". wp_continue.
-
-
-  lazymatch goal with
-  | |- environments.envs_entails _ (?φ (VStruct ?η)) =>
-      iExists _; iSplit ; first (iPureIntro; reflexivity)
-  end.
-  cbn; repeat iSplitL; try (iExists _; iSplit; first done); try done.
-  { (* Proof of the [sum] function.*)
-    iIntros(b1 b2 i1 i2).
-    wp_call. wp_continue. wp_continue.
-    wp_par.
-    - wp_use "Hr_val".
-      iIntros(?<-).
-      wp_call. wp_set_postcondition.
-    - wp_use "Hr_val".
-    - iIntros (v1 v2 -> <-). wp.
-      wp_call.
-      iPureIntro. unfold sum_pure;
-        destruct b1, b2; cbn;
-        by rewrite int.add_repr_repr. }
-  { (* Proof of the [flip] function. *)
-    iIntros(??); wp_call. wp_continue.
-    by wp_simp_using flip_body_spec. }
 Time Qed.
